*primes are odd

Factor.dfy
@@ -1,10 +1,38 @@
-function isEven(a: nat): bool
+predicate isEven(a: nat)
 {
     a % 2 == 0
 }
 
 type EvenInt = x: nat | isEven(x) witness 2
 type OddInt = x: nat | !isEven(x) witness 3
+
+function gcd(a: nat, b: nat): nat
+  requires a > 0 && b > 0
+{
+  if a == b
+    then a
+  else if a < b
+    then gcd(a, b-a)
+  else gcd(a-b, b)
+}
+
+predicate divider(a: nat, b:nat, k :nat)
+{
+    b == k * a
+}
+
+ghost predicate divides(a: nat, b:nat)
+    requires a > 0
+{
+    exists k: nat :: divider(a, b, k) 
+}
+
+ghost predicate prime(p: nat)
+{
+  (forall k: nat :: 1 < k < p - 1  ==> !divides(k, p)) && p >= 2 
+}
+
+type PrimeInt = x: nat | prime(x) witness 3
 
 function exp(x: nat, n: nat): int
 {
@@ -14,7 +42,7 @@ function exp(x: nat, n: nat): int
         x * exp(x, n-1)
 }
 
-method Factor(n: OddInt) returns (q: nat, e: nat)
+method Factor(n: PrimeInt) returns (q: nat, e: nat)
 requires n >= 3
 ensures n == q * exp(2, e) + 1
 ensures q >= 1
@@ -31,5 +59,39 @@ ensures !isEven(q)
     }
 }
 
+lemma EvenNumberIsDivisibleByTwoIndirect(n : nat) 
+    requires isEven(n)
+    requires n > 0
+    ensures divides(2, n)
+{   
+    if (!divides(2, n))
+    {
+         assert(!divides(2, n)); 
+         var k := n / 2; // wittness
+         assert(!divider(2, n, k));
+    }
+}
 
+lemma EvenNumberIsDivisibleByTwo(n : nat)
+    requires isEven(n)
+    requires n > 0
+    ensures divides(2, n)
+{
+    var k := n / 2; // wittness
+    assert(divider(2, n, k));
+    assert(divides(2, n)); 
+}
 
+lemma PrimeNumbersAreOdd(p: nat) 
+  requires prime(p)
+  requires p >=3
+  ensures(!isEven(p))
+{	
+    if (isEven(p))
+    {
+        assert(p % 2 == 0); 
+        EvenNumberIsDivisibleByTwo(p);
+        assert(divides(2, p));  
+        assert(!prime(p));
+    }
+}
